examples/nsl_pk/DY.Example.NSL.Protocol.Stateful.Proof.fst
@@ -16,7 +16,7 @@ open DY.Example.NSL.Protocol.Stateful
 
 /// The (local) state predicate.
 
-let state_predicate_nsl: local_state_predicate nsl_version = {
+let state_predicate_nsl: local_state_predicate nsl_session = {
   pred = (fun tr prin sess_id st ->
     match st with
     | InitiatorSentMsg1 bob n_a -> (
@@ -84,7 +84,7 @@ let event_predicate_nsl: event_predicate nsl_event =
 let all_sessions = [
   pki_tag_and_invariant;
   private_keys_tag_and_invariant;
-  (local_version_nsl_version.tag, local_state_predicate_to_local_bytes_state_predicate state_predicate_nsl);
+  (local_state_nsl_session.tag, local_state_predicate_to_local_bytes_state_predicate state_predicate_nsl);
 ]
 
 /// List of all local event predicates.
@@ -159,7 +159,7 @@ val send_msg1_proof:
     trace_invariant tr_out
   ))
 let send_msg1_proof tr global_sess_id alice sess_id =
-  match get_latest_version alice sess_id tr with
+  match get_state alice sess_id tr with
   | (Some (InitiatorSentMsg1 bob n_a), tr) -> (
     match get_public_key alice global_sess_id.pki (PkEnc "NSL.PublicKey") bob tr with
     | (None, tr) -> ()
@@ -200,7 +200,7 @@ val send_msg2_proof:
     trace_invariant tr_out
   ))
 let send_msg2_proof tr global_sess_id bob sess_id =
-  match get_latest_version bob sess_id tr with
+  match get_state bob sess_id tr with
   | (Some (ResponderSentMsg2 alice n_a n_b), tr) -> (
     match get_public_key bob global_sess_id.pki (PkEnc "NSL.PublicKey") alice tr with
     | (None, tr) -> ()
@@ -227,7 +227,7 @@ let prepare_msg3_proof tr global_sess_id alice sess_id msg_id =
     match get_private_key alice global_sess_id.private_keys (PkDec "NSL.PublicKey") tr with
     | (None, tr) -> ()
     | (Some sk_a, tr) -> (
-      match get_latest_version alice sess_id tr with
+      match get_state alice sess_id tr with
       | (Some (InitiatorSentMsg1 bob n_a), tr) -> (
         decode_message2_proof tr alice bob msg sk_a n_a
       )
@@ -245,7 +245,7 @@ val send_msg3_proof:
     trace_invariant tr_out
   ))
 let send_msg3_proof tr global_sess_id alice sess_id =
-  match get_latest_version alice sess_id tr with
+  match get_state alice sess_id tr with
   | (Some (InitiatorSentMsg3 bob n_a n_b), tr) -> (
     match get_public_key alice global_sess_id.pki (PkEnc "NSL.PublicKey") bob tr with
     | (None, tr) -> ()
@@ -289,7 +289,7 @@ let prepare_msg4 tr global_sess_id bob sess_id msg_id =
     match get_private_key bob global_sess_id.private_keys (PkDec "NSL.PublicKey") tr with
     | (None, tr) -> ()
     | (Some sk_b, tr) -> (
-      match get_latest_version bob sess_id tr with
+      match get_state bob sess_id tr with
       | (Some (ResponderSentMsg2 alice n_a n_b), tr) -> (
         decode_message3_proof tr alice bob msg sk_b n_b;
 
